MM2_PrefixSplice.v
@@ -22,7 +22,7 @@ From Undecidability.MinskyMachines Require Import MM2.
 Import MM2Notations.
 
 From kacc.MM2 Require Import Stepper.
-From kacc Require Import mm.
+From kacc Require Import CKA.Encoding.
 From kacc Require Import MM2.Simulator.
 From kacc Require Import EffectiveInseparability_MM2.
 
